fixed embarassing mistake in insert

list.v
@@ -46,5 +46,5 @@ nl: is_natlist []
 Inductive insert (x:nat) : list nat -> list nat -> Prop :=
 i_n : is_nat x -> insert x [] [x]
 | i_s : forall y: nat, forall ys: list nat, x <= y -> insert x (y :: ys) (x :: y :: ys)
-| i_c : forall y: nat, forall ys: list nat, forall rs: list nat, x > y -> insert x ys rs -> insert x (y :: ys) (x :: rs).
+| i_c : forall y: nat, forall ys: list nat, forall rs: list nat, y <= x-> insert x ys rs -> insert x (y :: ys) (y :: rs).
 
